{
 "cells": [
  {
   "cell_type": "markdown",
   "metadata": {},
   "source": [
    "# Initial-Value Problems\n",
    "\n",
    "This section focuses on analytical solutions for initial-value problems, meaning problems where we know the values of $y(t)$ and $\\frac{dy}{dt}$ at $t=0$ (or $y(x)$ and $\\frac{dy}{dx}$ at $x=0$): $y(0)$ and $y^{\\prime}(0)$."
   ]
  },
  {
   "cell_type": "markdown",
   "metadata": {},
   "source": [
    "## Equations with constant coefficents\n",
    "\n",
    "A common category of 2nd-order homogeneous ODEs are equations with constant coefficients, of the form:\n",
    "\\begin{equation}\n",
    "y^{\\prime\\prime} + a y^{\\prime} + by = 0\n",
    "\\end{equation}\n",
    "Note that these are unforced, and the right-hand side is zero.\n",
    "\n",
    "Solutions to these equations take the form $y(x) = e^{\\lambda x}$, and inserting this into the ODE gives us the characteristic equation\n",
    "\\begin{equation}\n",
    "\\lambda^2 + a \\lambda + b = 0\n",
    "\\end{equation}\n",
    "which we can solve to find the solution for given coefficients $a$ and $b$ and initial conditions. Depending on those coefficients and the solution to the characteristic equation, our solution can fall into one of three cases:\n",
    "\n",
    "* Real roots: $\\lambda_1$ and $\\lambda_2$. This is an **overdamped** system and the full solution takes the form\n",
    "\\begin{equation}\n",
    "y(x) = c_1 e^{\\lambda_1 x} + c_2 e^{\\lambda_2 x}\n",
    "\\end{equation}\n",
    "\n",
    "* Repeated roots: $\\lambda_1 = \\lambda_2 = \\lambda$. This is a **critically damped** system and the full solution is\n",
    "\\begin{equation}\n",
    "y(x) = c_1 e^{\\lambda x} + c_2 x e^{\\lambda x}\n",
    "\\end{equation}\n",
    "(Where does that second part come from, you might ask? Well, we know that $y_1$ is $e^{\\lambda x}$, but the second part cannot also be $e^{\\lambda x}$ because those are linearly dependent. So, we use *reduction of order* to find $y_2$, which is $x e^{\\lambda x}$.\n",
    "\n",
    "* Imaginary roots: $\\lambda = \\frac{-a}{2} \\pm \\beta i$, where $\\beta = \\frac{1}{2} \\sqrt{4b - a^2}$. This is an **underdamped** system and the solution takes the form\n",
    "\\begin{equation}\n",
    "y(x) = e^{-ax/2} \\left( c_1 \\sin \\beta x + c_2 \\cos \\beta x \\right)\n",
    "\\end{equation}\n",
    "\n",
    "Some examples:\n",
    "\n",
    "1. $y^{\\prime\\prime} + 3 y^{\\prime} + 2y = 0$\n",
    "\\begin{align}\n",
    "\\rightarrow \\lambda^2 + 3\\lambda + 2 &= 0 \\\\\n",
    "(\\lambda + 2)(\\lambda + 1) &= 0 \\\\\n",
    "\\lambda &= -2, -1 \\\\\n",
    "y(x) &= c_1 e^{-x} + c_2 e^{-2x}\n",
    "\\end{align}\n",
    "Then, we would use the initial conditions given for $y(0)$ and $y^{\\prime}(0)$ to find $c_1$ and $c_2$.\n",
    "\n",
    "2. $y^{\\prime\\prime} + 6 y^{\\prime} + 9y = 0$\n",
    "\\begin{align}\n",
    "\\rightarrow \\lambda^2 + 6\\lambda + 9 &= 0 \\\\\n",
    "(\\lambda + 3)(\\lambda + 3) &= 0 \\\\\n",
    "\\lambda &= -3 \\\\\n",
    "y(x) &= c_1 e^{-3x} + c_2 x e^{-3x}\n",
    "\\end{align}\n",
    "\n",
    "3. $y^{\\prime\\prime} + 6 y^{\\prime} + 25 y = 0$\n",
    "\\begin{align}\n",
    "\\rightarrow \\lambda^2 + 6\\lambda + 25 &= 0 \\\\\n",
    "\\lambda &= -3 \\pm 4i \\\\\n",
    "y(x) &= e^{-3x} \\left( c_1 \\sin 4x + c_2 \\cos 4x \\right)\n",
    "\\end{align}"
   ]
  },
  {
   "cell_type": "markdown",
   "metadata": {},
   "source": [
    "## Euler-Cauchy equations\n",
    "\n",
    "Euler-Cauchy equations are of the form\n",
    "\\begin{equation}\n",
    "x^2 y^{\\prime\\prime} + axy^{\\prime} + by = 0\n",
    "\\end{equation}\n",
    "\n",
    "Solutions take the form $y = x^m$, which when plugged into the ODE leads to a different characterisic equation to find $m$:\n",
    "\\begin{align}\n",
    "y &= x^m \\\\\n",
    "y^{\\prime} &= m x^{m-1} \\\\\n",
    "y^{\\prime\\prime} &= m (m-1) x^{m-2} \\\\\n",
    "\\rightarrow x^2 m (m-1) x^{m-2} + axmx^{m-1} + bx^m &= 0 \\\\\n",
    "m^2 + (a-1)m + b &= 0\n",
    "\\end{align}\n",
    "This is our new characteristic formula for these problems, and solving for the roots of this equation gives us $m$ and thus our general solution.\n",
    "\n",
    "Like equations with constant coefficients, we have three solution forms depending on the roots of the characteristic equation:\n",
    "\n",
    "* Real roots: $y(x) = c_1 x^{m_1} + c_2 x^{m_2}$\n",
    "* Repeated roots: $y(x) = c_1 x^m + c_2 x^m \\ln x$\n",
    "* Imaginary roots: $m = \\alpha \\pm \\beta i$, and $y(x) = x^{\\alpha} \\left[c_1 \\cos (\\beta \\ln x) + c_2 \\sin (\\beta \\ln x)\\right]$"
   ]
  },
  {
   "cell_type": "markdown",
   "metadata": {},
   "source": [
    "## Inhomogeneous 2nd-order ODEs\n",
    "\n",
    "Inhomogeneous, or forced, 2nd-order ODEs with constant coefficients take the form\n",
    "\\begin{equation}\n",
    "y^{\\prime\\prime} + a y^{\\prime} + by = F(t)\n",
    "\\end{equation}\n",
    "with initial conditions $y(0) = y_0$ and $y^{\\prime}(0) = y_0^{\\prime}$. Depending on the form of the forcing function $F(t)$, we can solve with techniques such as\n",
    "\n",
    " - the method of undetermined coefficients\n",
    " - variation of parameters\n",
    " - LaPlace transforms\n",
    "\n",
    "The solution in general to inhomogeneous ODEs includes two parts:\n",
    "\\begin{equation}\n",
    "y(t) = y_{\\text{H}} + y_{\\text{IH}} = c_1 y_1 + c_2 y_2 + y_{\\text{IH}} \\;,\n",
    "\\end{equation}\n",
    "where $y_{\\text{H}}$ is the solution from the equivalent homogeneous ODE $y^{\\prime\\prime} + a y^{\\prime} + b y = 0$.\n",
    "\n",
    "The forcing function $F(t)$ may be \n",
    "\n",
    " - continuous\n",
    " - periodic\n",
    " - aperiodic/discontinuous\n",
    " \n",
    "### Continuous $F(t)$: method of undetermined coefficients\n",
    "\n",
    "For continuous forcing functions, we have two solution methods: the method of undetermined coefficients, and variation of parameters. \n",
    "\n",
    "Generally you'll want to use the method of undetermined coefficients when possible, which depends on if $F(t)$ matches one of a set of functions. In that case, the form of the inhomogeneous solution $y_{\\text{IH}}(t)$ follows that of the forcing function $F(t)$, with one or more unknown constants:\n",
    "\n",
    "| $F(t)$        | $y_{\\text{IH}}(t)$ |\n",
    "| ------------- | :-------:|\n",
    "| constant      | $K$ |\n",
    "| $\\cos \\omega t$ | $K_1 \\cos \\omega t + K_2 \\sin \\omega t$ |\n",
    "| $\\sin \\omega t$ | $K_1 \\cos \\omega t + K_2 \\sin \\omega t$ |\n",
    "| $e^{-at}$ | $K e^{-at}$   |\n",
    "| $(A) t$   | $K_0 + K_1 t$ |\n",
    "| $t^n$     | $K_0 + K_1 t + K_2 t^2 + \\ldots + K_n t^n$|\n",
    "\n",
    "For combinations of these functions, we can combine functions; for example, given\n",
    "\\begin{align}\n",
    "F(t) &= e^{-at} \\cos \\omega t \\quad \\text{or} e^{-at} \\sin \\omega t \\\\\n",
    "y_{\\text{IH}} &= K_1 e^{-at} \\cos \\omega t + K_2 e^{-at} \\sin \\omega t\n",
    "\\end{align}\n",
    "(Note how in all the above cases how the inhomogeneous solution follows the functional form of the forcing function; for example, the exponential decay rate $a$ or the sinusoidal frequency $\\omega$ match.\n",
    "\n",
    "The method of undetermined coefficients works by plugging the candidate inhomogeneous solutionn $y_{\\text{IH}}$ into the full ODE, and solving for the constants (e.g., $K$)â€”but **not** from the initial conditions.\n",
    "\n",
    "For example, let's solve\n",
    "\\begin{equation}\n",
    "y^{\\prime\\prime} + 2y^{\\prime} + y = e^{-x}\n",
    "\\end{equation}\n",
    "with initial conditions $y(0) = y^{\\prime}(0) = 0$. First, we should find the solution to the homogeneous equation\n",
    "\\begin{equation}\n",
    "y^{\\prime\\prime} + 2y^{\\prime} + y = 0 \\;.\n",
    "\\end{equation}\n",
    "We can do this by using the associated characteristic formula\n",
    "\\begin{align}\n",
    "\\lambda^2 + 2 \\lambda + 1 &= 0 \\\\\n",
    "(\\lambda + 1)(\\lambda + 1) &= 0 \\\\\n",
    "\\rightarrow y_{\\text{H}} &= c_1 e^{-x} + c_2 x e^{-x}\n",
    "\\end{align}\n",
    "\n",
    "To find the inhomogeneous solution, we would look at the table above to find what matches the forcing function $e^{-x}$. Normally, we'd grab $K e^{-x}$, but that would not be linearly independent from the first part of the homogeneous solution $y_{\\text{H}}$. The same is true for $K x e^{-x}$, which is linearly dependent with the second part of $y_{\\text{H}}$, but $K x^2 e^{-x}$ works! Then, we just need to find $K$ by plugging this into the ODE:\n",
    "\\begin{align}\n",
    "y_{\\text{IH}} &= K x^2 e^{-x} \\\\\n",
    "y^{\\prime} &= K e^{-x} (2x - x^2) \\\\\n",
    "y^{\\prime\\prime} &= K e^{-x} (x^2 - 4x + 2) \\\\\n",
    "2 K &= 1 \\\\\n",
    "\\rightarrow K &= \\frac{1}{2} \\\\\n",
    "y_{\\text{IH}} &= \\frac{1}{2} x^2 e^{-x}\n",
    "\\end{align}\n",
    "Thus, the overall general solution is \n",
    "\\begin{equation}\n",
    "y(x) = c_1 e^{-x} + c_2 x e^{-x} + \\frac{1}{2} x^2 e^{-x}\n",
    "\\end{equation}\n",
    "and we would solve for the integration constants $c_1$ and $c_2$ using the initial conditions.\n",
    "\n",
    "Important points to remember:\n",
    "\n",
    "- The constants of the inhomogeneous solution $y_{\\text{IH}}$ come from the ODE, **not** the initial conditions.\n",
    "- Only solve for the integration constants $c_1$ and $c_2$ (part of the homogeneous solution) once you have the full general solution $y = c_1 y_1 + c_2 y_2 + y_{\\text{IH}}$.\n"
   ]
  },
  {
   "cell_type": "markdown",
   "metadata": {},
   "source": [
    "### Continuous $F(t)$: variation of parameters\n",
    "\n",
    "We have the variation of parameters approach to solve for inhomogeneous 2nd-order ODEs that are more general:\n",
    "\\begin{equation}\n",
    "y^{\\prime\\prime} + p(x) y^{\\prime} + q(x) y = r(x)\n",
    "\\end{equation}\n",
    "In this case, we can assume a solution $y(x) = y_1 u_1 + y_2 u_2$.\n",
    "\n",
    "The solution procedure is:\n",
    "\n",
    "1. Obtain $y_1$ and $y_2$ by solving the homogeneous equation: $y^{\\prime\\prime} + p(x) y^{\\prime} + q(x) y = 0$\n",
    "\n",
    "2. Solve for $u_1$ and $u_2$:\n",
    "\\begin{align}\n",
    "u_1 &= - \\int \\frac{y_2 r(x)}{W} dx + c_1 \\\\\n",
    "u_2 &= \\int \\frac{y_1 r(x)}{W} dx + c_2 \\\\\n",
    "W &= \\begin{vmatrix}\n",
    "y_1 & y_2\\\\ y_1^{\\prime} & y_2^{\\prime}\\\\\n",
    "\\end{vmatrix} = y_1 y_2^{\\prime} - y_2 y_1^{\\prime} \\;,\n",
    "\\end{align}\n",
    "where $W$ is the Wronksian.\n",
    "\n",
    "3. Then, we have the general solution:\n",
    "\\begin{align}\n",
    "y &= u_1 y_1 + u_2 y_2 \\\\\n",
    "&= \\left( -\\int \\frac{y_2 r(x)}{W} dx + c_1 \\right) y_1 + \\left( \\int \\frac{y_1 r(x)}{W} dx + c_2 \\right) y_2 \\;,\n",
    "\\end{align}\n",
    "where we solve for $c_1$ and $c_2$ using the two initial conditions.\n",
    "\n",
    "#### Example 1: variation of parameters\n",
    "\n",
    "First, let's try the same example we used for the method of undetermined coefficients above:\n",
    "\\begin{equation}\n",
    "y^{\\prime\\prime} + 2 y^{\\prime} + y = e^{-x}\n",
    "\\end{equation}\n",
    "We already found the homogeneous solution, so we know that $y_1 = e^{-x}$ and $y_2 = x e^{-x}$.\n",
    "Next, let's get the Wronksian, and then $u_1$ and $u_2$.\n",
    "\\begin{align}\n",
    "W &= \\begin{vmatrix} y_1 & y_2 \\\\ y_1^{\\prime} & y_2^{\\prime} \\end{vmatrix} = e^{-x} e^{-x}(1-x) - x e^{-x} (-e^{-x}) = e^{-2x} \\\\\n",
    "%\n",
    "u_1 &= -\\int \\frac{x e^{-x} e^{-x}}{e^{-2x}} dx + c_1 = -\\int x dx + c_1 = -\\frac{1}{2} x^2 + c_1 \\\\\n",
    "u_2 &= \\int \\frac{e^{-x} e^{-x}}{e^{-2x}} dx + c_2 = \\int dx + c_2 = x + c_2 \\\\\n",
    "y(x) &= \\left(-\\frac{1}{2} x^2 + c_1\\right) e^{-x} + (x + c_2) x e^{-x} \\\\\n",
    "\\end{align}\n",
    "After simplifying, we obtain the same solution as via the method of undetermined coefficients (but with a bit more work):\n",
    "\\begin{equation}\n",
    "y(x) = x_1 e^{-x} + c_2 x e^{-x} + \\frac{1}{2} x^2 e^{-x}\n",
    "\\end{equation}\n",
    "\n",
    "#### Example 2: variation of parameters\n",
    "\n",
    "Now let's try an example that we could *not* solve using the method of undetermined coefficients, with a forcing term that involves hyperbolic cosine (cosh); recall that $\\cosh(x) = \\frac{e^x + e^{-x}}{2}$.\n",
    "\\begin{equation}\n",
    "y^{\\prime\\prime} + 4 y^{\\prime} + 4y = \\cosh(x)\n",
    "\\end{equation}\n",
    "First, we need to find the homogeneous solution:\n",
    "\\begin{align}\n",
    "y^{\\prime\\prime} + 4 y^{\\prime} + 4y &= 0 \\\\\n",
    "\\lambda^2 + 4 \\lambda + 4 &= 0 \\\\\n",
    "\\rightarrow \\lambda &= -2\n",
    "\\end{align}\n",
    "So our homogeneous solution involves repeated roots:\n",
    "\\begin{equation}\n",
    "y_H = c_1 e^{-2x} + c_2 x e^{-2x}\n",
    "\\end{equation}\n",
    "where $y_1 = e^{-2x}$ and $y_2 = x e^{-2x}$.\n",
    "\n",
    "Then, we need to find $u_1$ and $u_2$, so let's get the Wronksian and then solve\n",
    "\\begin{align}\n",
    "W &= \\begin{vmatrix} y_1 & y_2 \\\\ y_1^{\\prime} & y_2^{\\prime} \\end{vmatrix} = e^{-2x} (e^{-2x}) (1 - 2x) - x e^{-2x}(-2 e^{-2x}) = e^{-4x} \\\\\n",
    "%\n",
    "u_1 &= - \\int \\frac{x e^{-2x} \\cosh x}{e^{-4x}} dx + c_1 = -\\int \\frac{x \\frac{1}{2}(e^x + e^{-x})}{e^{-2x}} dx + c_1 \\\\\n",
    " &= -\\frac{1}{2} \\int x (e^{3x} + e^x) dx + c_1 = -\\frac{1}{2} \\left[ \\frac{1}{9} e^{3x}(3x-1) + e^x(x-1) \\right] + c_1 \\\\\n",
    "u_1 &= -\\frac{1}{18} e^{3x}(3x-1) - \\frac{1}{2} e^x (x-1) + c_1 \\\\\n",
    "%\n",
    "u_2 &= \\int \\frac{e^{-2x} \\cosh x}{e^{-4x}} dx + c_2 = \\frac{1}{2} \\int e^{2x}(e^x + e^{-x}) dx + c_2 = \\frac{1}{2} \\int (e^{3x} + e^x) dx + c_2 \\\\ \n",
    "u_2 &= \\frac{1}{6} e^{3x} + \\frac{1}{2} e^x + c_2\n",
    "\\end{align}\n",
    "\n",
    "Then, when we put these all together, we get the full (complicated) solution:\n",
    "\\begin{equation}\n",
    "y(x) = \\left[ -\\frac{1}{18} e^{3x} (3x-1) - \\frac{1}{2} e^x (x-1) + c_1 \\right] e^{-2x} + \\left( \\frac{1}{6} e^{3x} + \\frac{1}{2} e^x + c_2 \\right) x e^{-2x}\n",
    "\\end{equation}"
   ]
  },
  {
   "cell_type": "code",
   "execution_count": null,
   "metadata": {},
   "outputs": [],
   "source": []
  }
 ],
 "metadata": {
  "kernelspec": {
   "display_name": "Matlab",
   "language": "matlab",
   "name": "matlab"
  },
  "language_info": {
   "codemirror_mode": "octave",
   "file_extension": ".m",
   "help_links": [
    {
     "text": "MetaKernel Magics",
     "url": "https://metakernel.readthedocs.io/en/latest/source/README.html"
    }
   ],
   "mimetype": "text/x-octave",
   "name": "matlab",
   "version": "0.16.11"
  }
 },
 "nbformat": 4,
 "nbformat_minor": 4
}
